pcuic/theories/PCUICValidity.v
@@ -1,20 +1,29 @@
 From Coq Require Import Bool String List Program BinPos Compare_dec Omega.
-From Template Require Import Template Ast Induction LiftSubst Typing WeakSubst.
-
+From Template Require Import utils.
+From PCUIC Require Import PCUICAst PCUICAstUtils PCUICInduction PCUICLiftSubst PCUICTyping PCUICWeakening.
+Existing Instance config.default_checker_flags.
 Lemma type_local_env_isdecl Σ n Γ :
-  forall isdecl : n < #|Γ|, type_local_env Σ Γ ->
+  forall isdecl : n < #|Γ|, All_local_env typing Σ Γ ->
   { Γ' : _ & { Γ'' : _ &
                     { _ : type_local_decl Σ Γ'' (safe_nth Γ (exist _ n isdecl)) &
                     Γ = Γ' ++ Γ'' /\ #|Γ'| = S n } } }.
 Proof. Admitted.
-         
-Theorem validity : env_prop (fun Σ Γ t T => type_local_env Σ Γ ->
-                                            isType Σ Γ T).
+
+Theorem validity : env_prop (fun Σ Γ t T => wf_local Σ Γ -> isType_or_Sort Σ Γ T).
 Proof.
   apply typing_ind_env; intros.
 
   - pose proof H as H0.
-    apply (type_local_env_isdecl _ _ _ isdecl) in H0 as [Γ' [Γ'' [H0 [-> <-]]]].
+    eapply (All_local_env_lookup X) in H.
+    red in H |- *. destruct decl as [na [b|] ty]. cbn -[skipn] in *.
+    forward H by auto with wf.
+    destruct H. left; destruct ty; simpl in i; depelim i. exact I.
+    right. destruct i as [u Hu].
+    exists u.
+
+
+
+    apply (type_local_env_isdecl _ _ _ H0) in X0. as [Γ' [Γ'' [H0 [-> <-]]]].
     destruct safe_nth. simpl in *.
     red in H0. simpl in H0. destruct decl_body. admit.
     destruct H0. exists x. 
